progress on trace definition

ListExtras.v
@@ -192,6 +192,12 @@ Proof.
     intros. apply H. right. assumption.
 Qed.
 
+Definition app_cons {A}
+  (a : A)
+  (l : list A)
+  : [a] ++ l = a :: l
+  := eq_refl.
+
 Lemma append_nodup_left {A}:
   forall (l1 l2 : list A), NoDup (l1 ++ l2) -> NoDup l1.
 Proof.
@@ -238,7 +244,7 @@ Qed.
 
 Require Import Streams.
 
-Definition stream_concat
+Definition stream_app
   {A : Type}
   (prefix : list A)
   (suffix : Stream A)
@@ -246,6 +252,22 @@ Definition stream_concat
   :=
   fold_right (@Cons A) suffix prefix.
 
+
+Definition stream_app_cons {A}
+  (a : A)
+  (l : Stream A)
+  : stream_app [a] l = Cons a l
+  := eq_refl.
+
+Lemma stream_app_assoc
+  {A : Type}
+  (l m : list A)
+  (n : Stream A)
+  : stream_app l (stream_app m n) = stream_app (l ++ m) n.
+Proof.
+  induction l; try reflexivity.
+  simpl. apply f_equal. assumption.
+Qed.
 
 
 (**
